Optimizations

ver2/optimizations_def.v
@@ -26,16 +26,19 @@ Import StackOpInstrs.
 Require Import FORVES.program.
 Import Program.
 
-Require Import symbolic_state_cmp_impl.
+Require Import FORVES.symbolic_state_cmp_impl.
 Import SymbolicStateCmpImpl.
 
-Require Import symbolic_state_eval_facts.
+Require Import FORVES.symbolic_state_eval_facts.
 Import SymbolicStateEvalFacts.
 
-Require Import misc.
+Require Import FORVES.valid_symbolic_state.
+Import ValidSymbolicState.
+
+Require Import FORVES.misc.
 Import Misc.
 
-Require Import eval_common.
+Require Import FORVES.eval_common.
 Import EvalCommon.
 
 Require Import List.
@@ -53,19 +56,42 @@ forall (sst: sstate) (sst': sstate) (b: bool),
 valid_sstate sst evm_stack_opm ->
 opt sst = (sst', b) ->
 (valid_sstate sst' evm_stack_opm /\ 
+ get_instk_height_sst sst = get_instk_height_sst sst' /\
  forall (st st': state), eval_sstate st sst  evm_stack_opm = Some st' ->
                          eval_sstate st sst' evm_stack_opm = Some st').
+                         
+
+Lemma optim_snd_same_height: forall sst sst' b opt,
+valid_sstate sst evm_stack_opm ->
+opt sst = (sst', b) ->
+optim_snd opt ->
+get_instk_height_sst sst = get_instk_height_sst sst'.
+Proof.
+intros sst sst' b opt Hvalid_sst Hopt Hopt_snd.
+unfold optim_snd in Hopt_snd.
+pose proof (Hopt_snd sst sst' b Hvalid_sst Hopt) as [_ Heval].
+destruct sst. destruct sst'.
+unfold eval_sstate in Heval.
+simpl in Heval.
+simpl.
+Admitted.
+
+                   
+
 
 (* sb2 preserves all the successful evaluations of sstack_val in sb1 *)
 Definition preserv_sbindings (sb1 sb2: sbindings) (maxidx: nat) 
-  (ops: stack_op_instr_map) : 
-Prop :=
+  (ops: stack_op_instr_map) (instk_height: nat) : Prop :=
+valid_bindings instk_height maxidx sb1 evm_stack_opm /\
+valid_bindings instk_height maxidx sb2 evm_stack_opm /\
 forall (sv : sstack_val) (stk : stack) (mem: memory) (strg: storage) 
   (ctx: context) (v: EVMWord),
+  instk_height = length stk ->
   eval_sstack_val sv stk mem strg ctx maxidx sb1 ops = Some v ->
   eval_sstack_val sv stk mem strg ctx maxidx sb2 ops = Some v.
 
 
+(* TODO: move to other file *)
 Lemma eval_sstack_def: forall (sstk: sstack) (maxidx: nat) (sb: sbindings) 
   (stk: stack) (mem: memory) (strg: storage) (ctx: context) 
   (ops: stack_op_instr_map),
@@ -79,29 +105,36 @@ Qed.
   
 (* sb2 preserves all the successful evaluations of sstack in sb1 *)  
 Lemma preserv_sbindings_sstack: 
-forall (sb1 sb2: sbindings) (maxidx: nat) (ops: stack_op_instr_map), 
-preserv_sbindings sb1 sb2 maxidx ops -> 
+forall (sb1 sb2: sbindings) (maxidx: nat) (ops: stack_op_instr_map) 
+  (instk_height: nat), 
+preserv_sbindings sb1 sb2 maxidx ops instk_height -> 
   forall (sstk: sstack) (stk stk': stack) (mem: memory) 
     (strg: storage) (ctx: context),
+  instk_height = length stk ->
   eval_sstack sstk maxidx sb1 stk mem strg ctx ops = Some stk' ->
   eval_sstack sstk maxidx sb2 stk mem strg ctx ops = Some stk'.
 Proof.
-intros sb1 sb2 maxidx ops Hpreserv sstk.
-revert sb1 sb2 maxidx ops Hpreserv.
+intros sb1 sb2 maxidx ops instk_height Hpreserv sstk.
+revert sb1 sb2 maxidx ops instk_height Hpreserv.
 induction sstk as [|sval r IH].
 - intuition.
-- intros sb1 sb2 maxid ops Hpreserv stk stk' mem strg ctx Heval.
+- intros sb1 sb2 maxid ops instk_height Hpreserv stk 
+    stk' mem strg ctx Hlen Heval.
   unfold preserv_sbindings in Hpreserv.
   unfold eval_sstack in Heval.
   unfold map_option in Heval.
   destruct (eval_sstack_val sval stk mem strg ctx maxid sb1 ops) as
     [v|] eqn: eq_eval_sval; try discriminate.
   rewrite <- map_option_ho in Heval.
-  pose proof (Hpreserv sval stk mem strg ctx v eq_eval_sval) as Heval_sval_sb2.
+  assert (Hpreserv_copy := Hpreserv).
+  destruct Hpreserv as [Hvalid_sb1 [Hvalid_sb2 Hpreserv]].
+  pose proof (Hpreserv sval stk mem strg ctx v Hlen eq_eval_sval) 
+    as Heval_sval_sb2.
   rewrite <- eval_sstack_def in Heval.
   destruct (eval_sstack r maxid sb1 stk mem strg ctx ops) as [rs_val|]
     eqn: eq_eval_rs; try discriminate.
-  apply IH with (sb2:=sb2) in eq_eval_rs as Heval_r_sb2; try assumption.
+  apply IH with (sb2:=sb2)(instk_height:=instk_height) in eq_eval_rs as 
+    Heval_r_sb2; try assumption.
   unfold eval_sstack.
   unfold map_option.
   rewrite -> Heval_sval_sb2.
@@ -112,28 +145,65 @@ induction sstk as [|sval r IH].
 Qed.
 
 
+Lemma valid_sbindings_rec: forall instk_height maxidx n smapv sb ops,
+valid_bindings instk_height maxidx ((n, smapv) :: sb) ops ->
+valid_bindings instk_height n sb ops.
+Proof.
+intros instk_height maxidx n smapv sb ops Hvalid.
+unfold valid_bindings in Hvalid.
+destruct Hvalid as [_ [_ Hvalid']].
+fold valid_bindings in Hvalid'.
+assumption.
+Qed.
 
 
 Lemma preserv_sbindings_ext: forall (sb1 sb2: sbindings) 
-  (maxidx: nat) (ops: stack_op_instr_map) (n: nat) (smapv: smap_value),
-preserv_sbindings sb1 sb2 maxidx ops ->
-preserv_sbindings ((n,smapv)::sb1) ((n,smapv)::sb2) maxidx ops.
+  (maxidx: nat) (ops: stack_op_instr_map) (n: nat) (smapv: smap_value)
+  (instk_height: nat),
+maxidx = S n ->
+valid_smap_value instk_height maxidx ops smapv ->
+preserv_sbindings sb1 sb2 n ops instk_height ->
+preserv_sbindings ((n,smapv)::sb1) ((n,smapv)::sb2) maxidx ops instk_height.
+Proof.
+(*
+intros sb1 sb2 maxidx ops n smapv instk_height Hmaxidx Hpreserv.
+unfold preserv_sbindings. 
+intros sv stk mem strg ctx v Hlen Hvalid_1 Hvalid_2 Heval.
+destruct sv as [val|var|fvar] eqn: eq_sv; try intuition.
+(* FreshVar case *)
+(*unfold eval_sstack_val. unfold eval_sstack_val'.
+unfold follow_in_smap.*)
+destruct (fvar =? n) eqn: eq_n_fvar.
+- (* Evaluate the same fvar in preserving sb1 and sb2 *)
+  admit.
+- rewrite -> eval_fvar_diff; try assumption.
+  rewrite -> eval_fvar_diff in Heval; try assumption.
+  unfold preserv_sbindings in Hpreserv.
+  apply Hpreserv; try intuition.
+  * apply valid_sbindings_rec with (maxidx:=maxidx)(smapv:=smapv).
+    assumption.
+  * apply valid_sbindings_rec with (maxidx:=maxidx)(smapv:=smapv).
+    assumption.  
+*)
 Admitted.
 
 (* sb2 preserves all the successful evaluations of smem in sb1 *)  
 Lemma preserv_sbindings_smemory:
-forall (sb1 sb2: sbindings) (maxidx: nat) (ops: stack_op_instr_map), 
-preserv_sbindings sb1 sb2 maxidx ops -> 
+forall (sb1 sb2: sbindings) (maxidx: nat) (ops: stack_op_instr_map)
+  (instk_height: nat), 
+preserv_sbindings sb1 sb2 maxidx ops instk_height -> 
   forall (smem: smemory) (stk: stack) (mem mem': memory) 
     (strg: storage) (ctx: context),
+  instk_height = length stk ->
   eval_smemory smem maxidx sb1 stk mem strg ctx ops = Some mem' ->
   eval_smemory smem maxidx sb2 stk mem strg ctx ops = Some mem'.
 Proof.
-intros sb1 sb2 maxidx ops Hpreserv smem.
-revert sb1 sb2 maxidx ops Hpreserv.
+intros sb1 sb2 maxidx ops instk_height Hpreserv smem.
+revert sb1 sb2 maxidx ops instk_height Hpreserv.
 induction smem as [|h r IH].
 - intuition.
-- intros sb1 sb2 maxidx ops Hpreserv stk mem mem' strg ctx Heval_mem.
+- intros sb1 sb2 maxidx ops instk_height Hpreserv stk mem mem' strg ctx 
+    Hlen Heval_mem.
   unfold eval_smemory in Heval_mem.
   unfold map_option in Heval_mem.
   unfold instantiate_memory_update in Heval_mem.
@@ -143,9 +213,10 @@ Admitted.
 (* sb2 preserves all the successful evaluations of sstorage in sb1 *)  
 Lemma preserv_sbindings_sstorage:
 forall (sb1 sb2: sbindings) (maxidx: nat)
-  (ops: stack_op_instr_map), 
-preserv_sbindings sb1 sb2 maxidx ops -> 
+  (ops: stack_op_instr_map) (instk_height: nat), 
+preserv_sbindings sb1 sb2 maxidx ops instk_height -> 
   forall (stk: stack) (sstrg: sstorage) (mem: memory) (strg strg': storage) (ctx: context),
+  instk_height = length stk ->
   eval_sstorage sstrg maxidx sb1 stk mem strg ctx ops = Some strg' ->
   eval_sstorage sstrg maxidx sb2 stk mem strg ctx ops = Some strg'.
 Proof.
@@ -155,17 +226,20 @@ Admitted.
 (* Changing a preseving sbinding in a sstate preserves successful evaluations *)
 Lemma preserv_sbindings_sstate :
 forall (sb1 sb2: sbindings) (maxidx: nat) 
-  (ops: stack_op_instr_map), 
-preserv_sbindings sb1 sb2 maxidx ops ->
-  forall (st st': state) (instk_height: nat) (sstk: sstack) (smem: smemory) 
+  (ops: stack_op_instr_map) (instk_height: nat), 
+preserv_sbindings sb1 sb2 maxidx ops instk_height ->
+valid_bindings instk_height maxidx sb1 evm_stack_opm ->
+valid_bindings instk_height maxidx sb2 evm_stack_opm ->
+  forall (st st': state) (sstk: sstack) (smem: smemory) 
   (sstrg: sstorage) (sctx : scontext),
+    instk_height = length (get_stack_st st) ->
     eval_sstate st (SymExState instk_height sstk smem sstrg sctx 
       (SymMap maxidx sb1)) ops = Some st' -> 
     eval_sstate st (SymExState instk_height sstk smem sstrg sctx 
       (SymMap maxidx sb2)) ops = Some st'.
 Proof.
-intros sb1 sb2 maxidx ops Hpr_sbind st st' instk_height sstk smem sstrg sctx
- Heval_sstate_sb1.
+intros sb1 sb2 maxidx ops instk_height Hpr_sbind Hvalid1 Hvalid2 st st' 
+  sstk smem sstrg sctx Heval_sstate_sb1.
 unfold eval_sstate in Heval_sstate_sb1.
 simpl in Heval_sstate_sb1.
 unfold eval_sstate. simpl.
@@ -174,20 +248,20 @@ destruct (instk_height =? length (get_stack_st st)) eqn: eq_instk_height;
 destruct (eval_sstack sstk maxidx sb1 (get_stack_st st) (get_memory_st st) 
   (get_storage_st st) (get_context_st st) ops) eqn: eq_eval_sstack; 
   try discriminate.
-apply preserv_sbindings_sstack with (sb2:=sb2) in eq_eval_sstack; 
-  try assumption.
+apply preserv_sbindings_sstack with (sb2:=sb2)(instk_height:=instk_height) in 
+  eq_eval_sstack; try assumption.
 rewrite -> eq_eval_sstack.
 destruct (eval_smemory smem maxidx sb1 (get_stack_st st) (get_memory_st st)
   (get_storage_st st) (get_context_st st) ops) eqn: eq_eval_smemory;
   try discriminate.
-apply preserv_sbindings_smemory with (sb2:=sb2) in eq_eval_smemory;
-  try assumption.
+apply preserv_sbindings_smemory with (sb2:=sb2)(instk_height:=instk_height) in 
+  eq_eval_smemory; try assumption.
 rewrite -> eq_eval_smemory.
 destruct (eval_sstorage sstrg maxidx sb1 (get_stack_st st) (get_memory_st st)
   (get_storage_st st) (get_context_st st) ops) eqn: eq_eval_sstorage;
   try discriminate.
-apply preserv_sbindings_sstorage with (sb2:=sb2) in eq_eval_sstorage;
-  try assumption.
+apply preserv_sbindings_sstorage with (sb2:=sb2)(instk_height:=instk_height) in 
+  eq_eval_sstorage; try assumption.
 rewrite -> eq_eval_sstorage.
 intuition.
 Qed.
@@ -198,14 +272,25 @@ Definition opt_smap_value_type := smap_value -> sstack_val_cmp_t -> sbindings ->
   nat -> nat -> stack_op_instr_map -> smap_value*bool.
 
 
+(* TODO: remove *)
+Lemma test: 
+valid_bindings 3 3 [(2,SymBasicVal (FreshVar 1));
+                    (1,SymBasicVal (InStackVar 2));
+                    (0,SymBasicVal (Val WZero))]
+               evm_stack_opm.
+Proof.
+simpl.
+intuition.
+Qed.
+
 (* 'opt' is sound if optimizing the head in a valid bindings (idx,val)::sb 
-   results in a valid bindings (idx,val') that preserves evaluations *)
+   results in a valid bindings (idx,val')::sb that preserves evaluations *)
 Definition opt_sbinding_snd (opt: opt_smap_value_type) :=
 forall (val val': smap_value) (fcmp: sstack_val_cmp_t) (sb: sbindings) 
   (maxidx: nat) (instk_height: nat) (idx: nat) (flag: bool),
 safe_sstack_val_cmp fcmp ->
 valid_bindings instk_height maxidx ((idx,val)::sb) evm_stack_opm ->
-opt val fcmp sb maxidx instk_height evm_stack_opm = (val', flag) ->
+opt val fcmp sb idx instk_height evm_stack_opm = (val', flag) ->
   valid_bindings instk_height maxidx ((idx,val')::sb) evm_stack_opm /\
   forall stk mem strg ctx v,
     instk_height = length stk ->
@@ -217,15 +302,15 @@ opt val fcmp sb maxidx instk_height evm_stack_opm = (val', flag) ->
 
 (* Applies smap value optimization to the first suitable entry in sbindings *)
 Fixpoint optimize_first_sbindings (opt_sbinding: opt_smap_value_type) 
-  (fcmp: sstack_val_cmp_t) (sb: sbindings) (maxid instk_height: nat) 
+  (fcmp: sstack_val_cmp_t) (sb: sbindings) (instk_height: nat) 
     : sbindings*bool :=
 match sb with
 | [] => (sb,false)
 | (n,val)::rs => 
-    match opt_sbinding val fcmp rs maxid instk_height evm_stack_opm with
+    match opt_sbinding val fcmp rs n instk_height evm_stack_opm with
     | (val', true) => ((n,val')::rs, true)
     | (val', false) => 
-        match (optimize_first_sbindings opt_sbinding fcmp rs maxid 
+        match (optimize_first_sbindings opt_sbinding fcmp rs
             instk_height) with 
         | (rs', flag) => ((n,val)::rs', flag)
         end
@@ -239,8 +324,15 @@ Lemma optimize_first_valid: forall (opt: opt_smap_value_type)
 safe_sstack_val_cmp fcmp ->
 opt_sbinding_snd opt ->
 valid_bindings instk_height maxid sb evm_stack_opm ->
-optimize_first_sbindings opt fcmp sb maxid instk_height = (sb', flag) ->
+optimize_first_sbindings opt fcmp sb instk_height = (sb', flag) ->
 valid_bindings instk_height maxid sb' evm_stack_opm.
+Proof.
+Admitted.
+
+
+Lemma valid_smap_value_succ: forall instk_height n ops smapv,
+valid_smap_value instk_height n ops smapv ->
+valid_smap_value instk_height (S n) ops smapv.
 Proof.
 Admitted.
 
@@ -253,8 +345,8 @@ forall (opt: opt_smap_value_type) (fcmp: sstack_val_cmp_t) (sb sb': sbindings)
 safe_sstack_val_cmp fcmp ->
 opt_sbinding_snd opt ->
 valid_bindings instk_height maxid sb evm_stack_opm ->
-optimize_first_sbindings opt fcmp sb maxid instk_height = (sb', flag) ->
-preserv_sbindings sb sb' maxid evm_stack_opm.
+optimize_first_sbindings opt fcmp sb instk_height = (sb', flag) ->
+preserv_sbindings sb sb' maxid evm_stack_opm instk_height.
 Proof.
 intros opt fcmp sb. revert opt fcmp.
 induction sb as [|h rsb IH].
@@ -270,43 +362,48 @@ induction sb as [|h rsb IH].
   assert (Hoptimize_first_sbindings_copy := Hoptimize_first_sbindings).
   assert (Hvalid_copy := Hvalid).
   unfold optimize_first_sbindings in Hoptimize_first_sbindings.
-  destruct (opt smapv fcmp rsb maxid instk_height evm_stack_opm) as [val' b] 
+  destruct (opt smapv fcmp rsb n instk_height evm_stack_opm) as [val' b] 
     eqn: eq_opt_val.
-  destruct b eqn: eq_b.
-  + (* Optimized first entry in sbindings *)
-    injection Hoptimize_first_sbindings as eq_sb' eq_flag'.
-    rewrite <- eq_sb'.
-    unfold preserv_sbindings.
-    intros sv stk mem strg ctx v Heval_sb.
-    destruct sv as [val|var|fvar] eqn: eq_sv; try intuition.
-    (* FreshVar fvar *)
-    destruct (fvar =? n) eqn: eq_fvar_n.
-    * rewrite -> PeanoNat.Nat.eqb_eq in eq_fvar_n.
-      rewrite -> eq_fvar_n.
-      rewrite -> eq_fvar_n in Heval_sb.
-    unfold opt_sbinding_snd in Hopt_sbinding_snd.
-    apply optimize_first_valid with (opt:=opt)(fcmp:=fcmp)(sb':=sb')(flag:=flag)
-      in Hvalid; try assumption.
-    pose proof (Hopt_sbinding_snd smapv val' fcmp rsb maxid instk_height n true
-      Hfcmp_snd Hvalid_copy eq_opt_val). 
-    (* TODO stk). mem). strg).  ctx v) as Hpres_fvar.
-          true Hfcmp_snd eq_opt_val n stk mem strg ctx v) as Hpres_fvar. *)
-    Admitted.
-(*    apply Hpres_fvar in Heval_sb.
-    assumption.
-    * rewrite -> eval_fvar_diff; try assumption.
-      rewrite -> eval_fvar_diff in Heval_sb; try assumption.
-  + (* Optimized the tail of the sbindings *)
-    fold optimize_first_sbindings in Hoptimize_first_sbindings.
-    destruct (optimize_first_sbindings opt fcmp rsb maxid instk_height) as
-      [rs' flag'] eqn: eq_optimize_first_rs.
-    injection Hoptimize_first_sbindings as eq_sb' eq_flag.
-    rewrite <- eq_sb'.
-    pose proof (IH opt fcmp rs' maxid instk_height flag' Hfcmp_snd
-      Hopt_sbinding_snd eq_optimize_first_rs) as Hpreserv_rs.
-    apply preserv_sbindings_ext.
-    assumption.
-Qed.*)
+  unfold preserv_sbindings.
+  split; try assumption.
+  split.
+  * (* valid_bindings instk_height maxid sb' evm_stack_opm *)
+    admit.
+  * destruct b eqn: eq_b.
+    + (* Optimized first entry in sbindings *)
+      injection Hoptimize_first_sbindings as eq_sb' eq_flag'.
+      rewrite <- eq_sb'.
+      unfold preserv_sbindings.
+      
+      intros sv stk mem strg ctx v Hlen Heval_sb.
+      destruct sv as [val|var|fvar] eqn: eq_sv; try intuition.
+      (* FreshVar fvar *)
+      destruct (fvar =? n) eqn: eq_fvar_n.
+      -- rewrite -> PeanoNat.Nat.eqb_eq in eq_fvar_n.
+         rewrite -> eq_fvar_n.
+         rewrite -> eq_fvar_n in Heval_sb.
+         unfold opt_sbinding_snd in Hopt_sbinding_snd.
+         pose proof (Hopt_sbinding_snd smapv val' fcmp rsb maxid instk_height n
+           true Hfcmp_snd Hvalid eq_opt_val) as [Hvalid2 Heval_imp].
+         pose proof (Heval_imp stk mem strg ctx v Hlen Heval_sb).
+         assumption.
+      -- rewrite -> eval_fvar_diff; try assumption.
+         rewrite -> eval_fvar_diff in Heval_sb; try assumption.
+    + (* Optimized the tail of the sbindings *)
+      fold optimize_first_sbindings in Hoptimize_first_sbindings.
+      destruct (optimize_first_sbindings opt fcmp rsb instk_height) as
+        [rs' flag'] eqn: eq_optimize_first_rs.
+      injection Hoptimize_first_sbindings as eq_sb' eq_flag.
+      rewrite <- eq_sb'.
+      unfold valid_bindings in Hvalid.
+      destruct Hvalid as [eq_maxid_n [Hvalid_smap Hvalid_rsb]].
+      fold valid_bindings in Hvalid_rsb.
+      pose proof (IH opt fcmp rs' n instk_height flag' Hfcmp_snd
+        Hopt_sbinding_snd Hvalid_rsb eq_optimize_first_rs) as Hpreserv_rs.
+      apply preserv_sbindings_ext; try intuition.
+      rewrite -> eq_maxid_n.
+      apply valid_smap_value_succ; try assumption.
+Admitted.
 
 
 
@@ -315,7 +412,7 @@ Definition optimize_first_sstate (opt: opt_smap_value_type)
   : sstate*bool :=
 match sst with 
 | SymExState instk_height sstk smem sstg sctx (SymMap maxid bindings) =>
-    match optimize_first_sbindings opt fcmp bindings maxid instk_height with
+    match optimize_first_sbindings opt fcmp bindings instk_height with
     | (bindings', flag) => 
         (SymExState instk_height sstk smem sstg sctx (SymMap maxid bindings'),
          flag)
@@ -325,17 +422,42 @@ end.
 Lemma optimize_first_sstate_valid: forall (opt: opt_smap_value_type) 
   (fcmp: sstack_val_cmp_t) (sst sst': sstate)
   (flag: bool),
-valid_sstate sst evm_stack_opm ->  
+valid_sstate sst evm_stack_opm ->
+opt_sbinding_snd opt ->
 optimize_first_sstate opt fcmp sst = (sst', flag) ->
 valid_sstate sst' evm_stack_opm.
 Proof.
+intros opt fcmp sst sst' flag Hvalid Hopt Hopt_first.
+unfold valid_sstate in Hvalid.
+destruct sst. destruct sm. simpl in Hvalid.
+destruct Hvalid as [valid_smap [valid_sstack [valid_smemory valid_sstorage]]].
+unfold optimize_first_sstate in Hopt_first.
+destruct (optimize_first_sbindings opt fcmp bindings instk_height) as
+  [bindings' flag'].
+injection Hopt_first as eq_sst' eq_flag'.
+rewrite <- eq_sst'.
+unfold valid_sstate. simpl.
+
+
+
+
 (* optimize_first_sstate does not change maxidx or stack_height, and does not
    change any fresh variable in the bindings, only one smap_value
    But I need some assumptions about the result of opt: it returns values
    that use smaller fresh variables or something like that *)
 Admitted.
 
-
+Lemma optimize_first_sstate_preserv: forall (opt: opt_smap_value_type) 
+  (fcmp: sstack_val_cmp_t) (sst sst': sstate)
+  (flag: bool),
+valid_sstate sst evm_stack_opm ->
+opt_sbinding_snd opt ->
+optimize_first_sstate opt fcmp sst = (sst', flag) ->
+ get_instk_height_sst sst = get_instk_height_sst sst' /\
+ forall (st st': state), eval_sstate st sst  evm_stack_opm = Some st' ->
+                         eval_sstate st sst' evm_stack_opm = Some st'.
+Proof.
+Admitted.
 
 
 
@@ -364,6 +486,14 @@ match val with
     (val, false)
 | _ => (val, false)
 end.
+
+(*
+Check (
+optimize_add_0_sbinding 
+  (SymOp ADD [(Val WZero); (Val WOne)])
+  compare_sstack_val  
+).
+*)
 
 (* Macro to reduce the next proof *)
 Ltac inject_rw H eqname:= 
@@ -448,111 +578,145 @@ eval_sstack_val' maxidx arg2 stk mem strg ctx maxidx sb ops.
 Proof.
 Admitted.
 
+Search (eval_sstack_val').
+
 Lemma optimize_add_0_sbinding_snd:
 opt_sbinding_snd optimize_add_0_sbinding.
 Proof.
+(*
 unfold opt_sbinding_snd.
-intros val val' fcmp sb maxidx instk_height flag Hsafe_sstack_val_cmp
-  Hoptm_add_0_sbinding idx stk mem strg ctx v Heval_orig.
-unfold optimize_add_0_sbinding in Hoptm_add_0_sbinding.
-destruct val as [vv|vv|label args|offset smem|key sstrg|offset seze smem]
-  eqn: eq_val; try inject_rw Hoptm_add_0_sbinding eq_val'.
-(* SymOp label args *)
-destruct label; try inject_rw Hoptm_add_0_sbinding eq_val'.
-destruct args as [|arg1 r1] eqn: eq_args; 
-  try inject_rw Hoptm_add_0_sbinding eq_val'.
-destruct r1 as [|arg2 r2] eqn: eq_r1; 
-  try inject_rw Hoptm_add_0_sbinding eq_val'.
-destruct r2 as [|arg3 r3] eqn: eq_r2; 
-  try inject_rw Hoptm_add_0_sbinding eq_val'.
-destruct (fcmp arg1 (Val WZero) maxidx sb maxidx sb instk_height) 
-  eqn: fcmp_arg1_zero.
-- (* arg1 ~ WZero *)
-  injection Hoptm_add_0_sbinding as eq_val' _. 
-  rewrite <- eq_val'.
-  unfold eval_sstack_val in Heval_orig. simpl in Heval_orig.
-  rewrite -> PeanoNat.Nat.eqb_refl in Heval_orig.
-  simpl in Heval_orig.
-  destruct (eval_sstack_val' maxidx arg1 stk mem strg ctx idx sb evm_stack_opm)
-    as [varg1|] eqn: eval_arg1; try discriminate.
-  destruct (eval_sstack_val' maxidx arg2 stk mem strg ctx idx sb evm_stack_opm)
-    as [varg2|] eqn: eval_arg2; try discriminate.
-  unfold safe_sstack_val_cmp in Hsafe_sstack_val_cmp.
-  (* fake lemmas for now, should be premises obtained somewhere *)
-  pose proof (fake1 instk_height maxidx arg1) as cfake1.
-  pose proof (fake1 instk_height maxidx (Val WZero)) as cfake2.
-  pose proof (fake2 instk_height maxidx sb evm_stack_opm) as cfake3.
-  pose proof (fake3 instk_height stk) as cfake4.
-  (* *)
-  pose proof (Hsafe_sstack_val_cmp arg1 (Val WZero) maxidx sb maxidx sb 
-    instk_height evm_stack_opm cfake1 cfake2 cfake3 cfake3
-    fcmp_arg1_zero stk mem strg ctx) as eq_eval_arg1.
-  rewrite -> eval_sstack_val_const in eq_eval_arg1.
-  unfold eval_sstack_val in eq_eval_arg1.
-  pose proof (Gt.gt_Sn_n maxidx) as eq_gt_succ.
-  pose proof (eval_sstack_val'_succ (S maxidx) instk_height arg1 stk mem
-    strg ctx maxidx sb evm_stack_opm cfake4 cfake1 cfake3 eq_gt_succ) as
-      [vv eq_eval'_arg1].
-  pose proof (eval_sstack_val'_preserved_when_depth_extended maxidx idx sb
-    arg1 varg1 stk mem strg ctx evm_stack_opm eval_arg1) as Heval'_arg1.
-  apply eval'_maxidx_indep with (m:=maxidx) in Heval'_arg1.
-  rewrite -> eq_eval'_arg1 in Heval'_arg1.
-  rewrite -> eq_eval_arg1 in eq_eval'_arg1.
-  injection eq_eval'_arg1 as eq_vv.
-  injection Heval'_arg1 as eq_varg1.
-  rewrite <- eq_vv in eq_varg1.
-  rewrite <- eq_varg1 in Heval_orig.
-  rewrite -> evm_add_zero_l in Heval_orig.
-  injection Heval_orig as eq_v.
-  rewrite <- eq_v.
-  unfold eval_sstack_val.
-  rewrite -> eval_freshv_top.
-  rewrite -> eval'_maxidx_indep with (n:=idx)(v:=varg2); try intuition.
-- destruct (fcmp arg2 (Val WZero) maxidx sb maxidx sb instk_height)
-  eqn: fcmp_arg2_zero; try inject_rw Hoptm_add_0_sbinding eq_val'.
-  (* arg2 ~ WZero *)
-  injection Hoptm_add_0_sbinding as eq_val' _. 
-  
-  rewrite <- eq_val'.
-  unfold eval_sstack_val in Heval_orig. simpl in Heval_orig.
-  rewrite -> PeanoNat.Nat.eqb_refl in Heval_orig.
-  simpl in Heval_orig.
-  destruct (eval_sstack_val' maxidx arg1 stk mem strg ctx idx sb evm_stack_opm)
-    as [varg1|] eqn: eval_arg1; try discriminate.
-  destruct (eval_sstack_val' maxidx arg2 stk mem strg ctx idx sb evm_stack_opm)
-    as [varg2|] eqn: eval_arg2; try discriminate.
-  unfold safe_sstack_val_cmp in Hsafe_sstack_val_cmp.
-  (* fake lemmas for now, should be premises obtained somewhere *)
-  pose proof (fake1 instk_height maxidx arg2) as cfake1.
-  pose proof (fake1 instk_height maxidx (Val WZero)) as cfake2.
-  pose proof (fake2 instk_height maxidx sb evm_stack_opm) as cfake3.
-  pose proof (fake3 instk_height stk) as cfake4.
-  (****)
-  pose proof (Hsafe_sstack_val_cmp arg2 (Val WZero) maxidx sb maxidx sb 
-    instk_height evm_stack_opm cfake1 cfake2 cfake3 cfake3
-    fcmp_arg2_zero stk mem strg ctx) as eq_eval_arg2.
-  rewrite -> eval_sstack_val_const in eq_eval_arg2.
-  unfold eval_sstack_val in eq_eval_arg2.
-  pose proof (Gt.gt_Sn_n maxidx) as eq_gt_succ.
-  pose proof (eval_sstack_val'_succ (S maxidx) instk_height arg2 stk mem
-    strg ctx maxidx sb evm_stack_opm cfake4 cfake1 cfake3 eq_gt_succ) as
-      [vv eq_eval'_arg2].
-  pose proof (eval_sstack_val'_preserved_when_depth_extended maxidx idx sb
-    arg2 varg2 stk mem strg ctx evm_stack_opm eval_arg2) as Heval'_arg2.
-  apply eval'_maxidx_indep with (m:=maxidx) in Heval'_arg2.
-  rewrite -> eq_eval'_arg2 in Heval'_arg2.
-  rewrite -> eq_eval_arg2 in eq_eval'_arg2.
-  injection eq_eval'_arg2 as eq_vv.
-  injection Heval'_arg2 as eq_varg2.
-  rewrite <- eq_vv in eq_varg2.
-  rewrite <- eq_varg2 in Heval_orig.
-  rewrite -> evm_add_zero_r in Heval_orig.
-  injection Heval_orig as eq_v.
-  rewrite <- eq_v.
-  unfold eval_sstack_val.
-  rewrite -> eval_freshv_top.
-  rewrite -> eval'_maxidx_indep with (n:=idx)(v:=varg1); try intuition.
-Qed.
+intros val val' fcmp sb maxidx instk_height idx flag Hsafe_sstack_val_cmp
+  Hvalid Hoptm_add_0_sbinding.
+split.
+- (* valid_sbindings *)
+  simpl. simpl in Hvalid.
+  destruct Hvalid as [Hmaxidx [Hvalid_smap_value_val Hvalid_sb]].
+  split; try split; try assumption.
+  (* use general lemma for every "safe" optimization *)
+  admit.
+- (* evaluation is preserved *) 
+  intros stk mem strg ctx v Hlen Heval_orig.
+  assert (Hlen2 := Hlen).
+  rewrite -> Hlen in Hlen2.
+  rewrite <- Hlen in Hlen2 at 2.
+  unfold optimize_add_0_sbinding in Hoptm_add_0_sbinding.
+  destruct val as [vv|vv|label args|offset smem|key sstrg|offset seze smem]
+    eqn: eq_val; try inject_rw Hoptm_add_0_sbinding eq_val'.
+  (* SymOp label args *)
+  destruct label; try inject_rw Hoptm_add_0_sbinding eq_val'.
+  destruct args as [|arg1 r1] eqn: eq_args; 
+    try inject_rw Hoptm_add_0_sbinding eq_val'.
+  destruct r1 as [|arg2 r2] eqn: eq_r1; 
+    try inject_rw Hoptm_add_0_sbinding eq_val'.
+  destruct r2 as [|arg3 r3] eqn: eq_r2; 
+    try inject_rw Hoptm_add_0_sbinding eq_val'.
+  destruct (fcmp arg1 (Val WZero) maxidx sb maxidx sb instk_height) 
+    eqn: fcmp_arg1_zero.
+  + (* arg1 ~ WZero *)
+    injection Hoptm_add_0_sbinding as eq_val' _. 
+    rewrite <- eq_val'.
+    unfold eval_sstack_val in Heval_orig. simpl in Heval_orig.
+    rewrite -> PeanoNat.Nat.eqb_refl in Heval_orig.
+    simpl in Heval_orig.
+    destruct (eval_sstack_val' maxidx arg1 stk mem strg ctx idx sb evm_stack_opm)
+      as [varg1|] eqn: eval_arg1; try discriminate.
+    destruct (eval_sstack_val' maxidx arg2 stk mem strg ctx idx sb evm_stack_opm)
+      as [varg2|] eqn: eval_arg2; try discriminate.
+    unfold safe_sstack_val_cmp in Hsafe_sstack_val_cmp.
+    
+    (* fake lemmas for now, should be premises obtained somewhere *)
+    (* TODO *) 
+    unfold valid_bindings in Hvalid.
+    destruct Hvalid as [eq_maxid [Hvalid_smap_value Hvalid_bindings_sb]].
+    unfold valid_smap_value in Hvalid_smap_value.
+    unfold valid_stack_op_instr in Hvalid_smap_value.
+    simpl in Hvalid_smap_value.
+    destruct (Hvalid_smap_value) as [_ [Hvalid_arg1 [Hvalid_arg2 _ ]]].
+    fold valid_bindings in Hvalid_bindings_sb.
+    
+    pose proof (fake1 instk_height maxidx arg1) as cfake1.
+    pose proof (fake1 instk_height maxidx (Val WZero)) as cfake2.
+    pose proof (fake2 instk_height maxidx sb evm_stack_opm) as cfake3.
+    (* TODO *) 
+    pose proof (Hsafe_sstack_val_cmp arg1 arg2 idx sb idx sb 
+      instk_height evm_stack_opm Hvalid_arg1 Hvalid_arg2 Hvalid_bindings_sb
+      Hvalid_bindings_sb). cfake1 cfake2 cfake3 cfake3
+      fcmp_arg1_zero stk mem strg ctx Hlen2) as eq_eval_arg1.
+    pose proof (Hsafe_sstack_val_cmp arg1 (Val WZero) maxidx sb maxidx sb 
+      instk_height evm_stack_opm cfake1 cfake2 cfake3 cfake3
+      fcmp_arg1_zero stk mem strg ctx Hlen2) as eq_eval_arg1.
+    destruct eq_eval_arg1 as [v1 [eq_eval_arg1 eq_eval_zero]].
+    rewrite -> eval_sstack_val_const in eq_eval_zero.
+    injection eq_eval_zero as eq_v1_zero.
+    rewrite <- eq_v1_zero in eq_eval_arg1.
+    unfold eval_sstack_val in eq_eval_arg1.
+    pose proof (Gt.gt_Sn_n maxidx) as eq_gt_succ.
+    pose proof (eval_sstack_val'_succ (S maxidx) instk_height arg1 stk mem
+      strg ctx maxidx sb evm_stack_opm Hlen cfake1 cfake3 eq_gt_succ) as
+        [vv eq_eval'_arg1].
+    pose proof (eval_sstack_val'_preserved_when_depth_extended maxidx idx sb
+      arg1 varg1 stk mem strg ctx evm_stack_opm eval_arg1) as Heval'_arg1.
+    apply eval'_maxidx_indep with (m:=maxidx) in Heval'_arg1.
+    rewrite -> eq_eval'_arg1 in Heval'_arg1.
+    rewrite -> eq_eval_arg1 in eq_eval'_arg1.
+    injection eq_eval'_arg1 as eq_vv.
+    injection Heval'_arg1 as eq_varg1.
+    rewrite <- eq_vv in eq_varg1.
+    rewrite <- eq_varg1 in Heval_orig.
+    rewrite -> evm_add_zero_l in Heval_orig.
+    injection Heval_orig as eq_v.
+    rewrite <- eq_v.
+    unfold eval_sstack_val.
+    rewrite -> eval_freshv_top.
+    apply eval'_maxidx_indep with (n:=idx).
+    assumption. 
+  * admit.
+    (*destruct (fcmp arg2 (Val WZero) maxidx sb maxidx sb instk_height)
+    eqn: fcmp_arg2_zero; try inject_rw Hoptm_add_0_sbinding eq_val'.
+    (* arg2 ~ WZero *)
+    injection Hoptm_add_0_sbinding as eq_val' _. 
+    
+    rewrite <- eq_val'.
+    unfold eval_sstack_val in Heval_orig. simpl in Heval_orig.
+    rewrite -> PeanoNat.Nat.eqb_refl in Heval_orig.
+    simpl in Heval_orig.
+    destruct (eval_sstack_val' maxidx arg1 stk mem strg ctx idx sb evm_stack_opm)
+      as [varg1|] eqn: eval_arg1; try discriminate.
+    destruct (eval_sstack_val' maxidx arg2 stk mem strg ctx idx sb evm_stack_opm)
+      as [varg2|] eqn: eval_arg2; try discriminate.
+    unfold safe_sstack_val_cmp in Hsafe_sstack_val_cmp.
+    (* fake lemmas for now, should be premises obtained somewhere *)
+    pose proof (fake1 instk_height maxidx arg2) as cfake1.
+    pose proof (fake1 instk_height maxidx (Val WZero)) as cfake2.
+    pose proof (fake2 instk_height maxidx sb evm_stack_opm) as cfake3.
+    pose proof (fake3 instk_height stk) as cfake4.
+    (****)
+    pose proof (Hsafe_sstack_val_cmp arg2 (Val WZero) maxidx sb maxidx sb 
+      instk_height evm_stack_opm cfake1 cfake2 cfake3 cfake3
+      fcmp_arg2_zero stk mem strg ctx) as eq_eval_arg2.
+    rewrite -> eval_sstack_val_const in eq_eval_arg2.
+    unfold eval_sstack_val in eq_eval_arg2.
+    pose proof (Gt.gt_Sn_n maxidx) as eq_gt_succ.
+    pose proof (eval_sstack_val'_succ (S maxidx) instk_height arg2 stk mem
+      strg ctx maxidx sb evm_stack_opm cfake4 cfake1 cfake3 eq_gt_succ) as
+        [vv eq_eval'_arg2].
+    pose proof (eval_sstack_val'_preserved_when_depth_extended maxidx idx sb
+      arg2 varg2 stk mem strg ctx evm_stack_opm eval_arg2) as Heval'_arg2.
+    apply eval'_maxidx_indep with (m:=maxidx) in Heval'_arg2.
+    rewrite -> eq_eval'_arg2 in Heval'_arg2.
+    rewrite -> eq_eval_arg2 in eq_eval'_arg2.
+    injection eq_eval'_arg2 as eq_vv.
+    injection Heval'_arg2 as eq_varg2.
+    rewrite <- eq_vv in eq_varg2.
+    rewrite <- eq_varg2 in Heval_orig.
+    rewrite -> evm_add_zero_r in Heval_orig.
+    injection Heval_orig as eq_v.
+    rewrite <- eq_v.
+    unfold eval_sstack_val.
+    rewrite -> eval_freshv_top.
+    rewrite -> eval'_maxidx_indep with (n:=idx)(v:=varg1); try intuition.*)
+*)    
+Admitted.
 
 
 (* *)
@@ -566,6 +730,29 @@ optim_snd (optimize_add_0 fcmp).
 Proof.
 intros fcmp Hsafe_fcmp.
 unfold optim_snd. intros sst sst' b Hvalid_sst Hoptim.
+unfold optimize_add_0 in Hoptim.
+split.
+- pose proof (optimize_first_sstate_valid optimize_add_0_sbinding fcmp sst 
+    sst' b Hvalid_sst optimize_add_0_sbinding_snd Hoptim).
+  assumption.
+- pose proof (optimize_first_sstate_preserv optimize_add_0_sbinding fcmp sst 
+    sst' b Hvalid_sst optimize_add_0_sbinding_snd Hoptim) as [Hinstk Heval].
+  split; try assumption.
+(*
+unfold optimize_add_0 in Hoptim. 
+destruct sst as [instk_height sstk smem sstg sctx sm].
+unfold optimize_first_sstate in Hoptim.
+destruct sm as [maxid bindings].
+destruct (optimize_first_sbindings optimize_add_0_sbinding fcmp bindings
+  instk_height) as [bindings' flag].
+injection Hoptim as eq_sst' eq_b.
+rewrite <- eq_sst'. simpl.
+
+split.
+- (* valid_sstate sst' evm_stack_opm *)
+  admit.
+- split.
+  + 
 unfold optimize_add_0 in Hoptim.
 split.
 - apply optimize_first_sstate_valid with (opt:=optimize_add_0_sbinding)
@@ -584,8 +771,8 @@ split.
     optimize_add_0_sbinding_snd eq_opt_first) as Hpreserves.
   pose proof (preserv_sbindings_sstate bindings bindings' maxid evm_stack_opm
     Hpreserves st st' instk_height sstk smem sstg sctx).
-  intuition.
-Qed.  
+  intuition.*)
+Qed.
 
 
 End Optimizations_Def.
